use sep_auto instead of hoare_triples

Weidenbach_Book/Array_Array_List.thy
@@ -10,7 +10,11 @@ fun heap_list_all :: "('a \<Rightarrow> 'b \<Rightarrow> assn) \<Rightarrow> 'a 
 definition heap_list_all_nth:: "('a \<Rightarrow> 'b \<Rightarrow> assn) \<Rightarrow> nat list \<Rightarrow>  'a list \<Rightarrow> 'b list \<Rightarrow> assn" where
   \<open>heap_list_all_nth R is xs ys = foldr (op *) (map (\<lambda>i. R (xs ! i) (ys ! i)) is) emp\<close>
 
-lemma heap_list_all_nth_emty[simp]: \<open>heap_list_all_nth R [] [] [] = emp\<close>
+lemma heap_list_all_nth_emty[simp]: \<open>heap_list_all_nth R [] xs ys = emp\<close>
+  unfolding heap_list_all_nth_def by auto
+
+lemma heap_list_all_nth_Cons:
+  \<open>heap_list_all_nth R (a # is') xs ys = R (xs ! a) (ys ! a) * heap_list_all_nth R is' xs ys\<close>
   unfolding heap_list_all_nth_def by auto
 
 lemma heap_list_all_heap_list_all_nth:
@@ -34,12 +38,128 @@ proof (induction R xs ys rule: heap_list_all.induct)
     using IH unfolding 1 by auto
 qed auto
 
-definition arrayO:: \<open>('a \<Rightarrow> 'b::heap \<Rightarrow> assn) \<Rightarrow> 'a list \<Rightarrow> 'b array \<Rightarrow> assn\<close> where
-  \<open>arrayO R' xs axs \<equiv> \<exists>\<^sub>A p. array_assn id_assn p axs * heap_list_all R' xs p\<close>
+lemma heap_list_all_nth_single: \<open>heap_list_all_nth R [a] xs ys = R (xs ! a) (ys ! a)\<close>
+  by (auto simp: heap_list_all_nth_def)
+
+lemma heap_list_all_nth_mset_eq:
+  assumes \<open>mset is = mset is'\<close>
+  shows \<open>heap_list_all_nth R is xs ys = heap_list_all_nth R is' xs ys\<close>
+  using assms
+proof (induction "is'" arbitrary: "is")
+  case Nil
+  then show ?case by auto
+next
+  case (Cons a is') note IH = this(1) and eq_is = this(2)
+  from eq_is have \<open>a \<in> set is\<close>
+    by (fastforce dest: mset_eq_setD)
+  then obtain ixs iys where
+    "is": \<open>is = ixs @ a # iys\<close>
+    using eq_is  by (meson split_list)
+  then have H: \<open>heap_list_all_nth R (ixs @ iys) xs ys = heap_list_all_nth R is' xs ys\<close>
+    using IH[of \<open>ixs @ iys\<close>] eq_is by auto
+  have H': \<open>heap_list_all_nth R (ixs @ a # iys) xs ys = heap_list_all_nth R (a # ixs @ iys) xs ys\<close>
+    for xs ys
+    by (induction ixs)(auto simp: heap_list_all_nth_Cons star_aci(3))
+  show ?case
+    using H[symmetric] by (auto simp: heap_list_all_nth_Cons "is" H')
+qed
 
 lemma heap_list_add_same_length:
   \<open>h \<Turnstile> heap_list_all R' xs p \<Longrightarrow> length p = length xs\<close>
   by (induction R' xs p arbitrary: h rule: heap_list_all.induct) (auto elim!: mod_starE)
+
+lemma heap_list_all_nth_Suc:
+  assumes a: \<open>a > 1\<close>
+  shows \<open>heap_list_all_nth R [Suc 0..<a] (x # xs) (y # ys) =
+    heap_list_all_nth R [0..<a-1] xs ys\<close>
+proof -
+  have upt: \<open>[0..< a] = 0 # [1..< a]\<close>
+    using a by (simp add: upt_rec)
+  have upt_map_Suc: \<open>[Suc 0..<a] = map Suc [0..< a-1]\<close>
+    using a by (auto simp: map_Suc_upt)
+  have map: \<open>(map (\<lambda>i. R ((x # xs) ! i) ((y # ys) ! i)) [Suc 0..<a]) =
+    (map (\<lambda>i. R (xs ! i) (ys ! i)) [0..<a-1])\<close>
+    unfolding upt_map_Suc map_map by auto
+  show ?thesis
+    unfolding heap_list_all_nth_def unfolding map ..
+qed
+
+lemma heap_list_all_nth_append:
+  \<open>heap_list_all_nth R (is @ is') xs ys = heap_list_all_nth R is xs ys * heap_list_all_nth R is' xs ys\<close>
+  by (induction "is") (auto simp: heap_list_all_nth_Cons star_aci)
+
+lemma heap_list_all_heap_list_all_nth_eq:
+  \<open>heap_list_all R xs ys = heap_list_all_nth R [0..< length xs] xs ys * \<up>(length xs = length ys)\<close>
+  by (induction R xs ys rule: heap_list_all.induct)
+    (auto simp del: upt_Suc simp: upt_rec[of 0] heap_list_all_nth_single star_aci(3)
+      heap_list_all_nth_Cons heap_list_all_nth_Suc)
+
+lemma heap_list_all_nth_remove1: \<open>i \<in> set is \<Longrightarrow>
+  heap_list_all_nth R is xs ys = R (xs ! i) (ys ! i) * heap_list_all_nth R (remove1 i is) xs ys\<close>
+  using heap_list_all_nth_mset_eq[of \<open>is\<close> \<open>i # remove1 i is\<close>]
+  by (auto simp: heap_list_all_nth_Cons)
+
+definition arrayO:: \<open>('a \<Rightarrow> 'b::heap \<Rightarrow> assn) \<Rightarrow> 'a list \<Rightarrow> 'b array \<Rightarrow> assn\<close> where
+  \<open>arrayO R' xs axs \<equiv> \<exists>\<^sub>A p. array_assn id_assn p axs * heap_list_all R' xs p\<close>
+
+definition arrayO_except:: \<open>('a \<Rightarrow> 'b::heap \<Rightarrow> assn) \<Rightarrow> nat list \<Rightarrow> 'a list \<Rightarrow> 'b array \<Rightarrow> _ \<Rightarrow> assn\<close> where
+  \<open>arrayO_except R' is xs axs f \<equiv>
+     \<exists>\<^sub>A p. array_assn id_assn p axs * heap_list_all_nth R' (fold remove1 is [0..<length xs]) xs p *
+    \<up> (length xs = length p) * f p\<close>
+
+lemma arrayO_except_array0: \<open>arrayO_except R [] xs asx (\<lambda>_. emp) = arrayO R xs asx\<close>
+proof -
+  have \<open>(h \<Turnstile> array_assn id_assn p asx * heap_list_all_nth R [0..<length xs] xs p \<and> length xs = length p) =
+    (h \<Turnstile> array_assn id_assn p asx * heap_list_all R xs p)\<close> (is \<open>?a = ?b\<close>) for h p
+  proof (rule iffI)
+    assume ?a
+    then show ?b
+      by (auto simp: (* heap_list_add_same_length *) heap_list_all_heap_list_all_nth)
+  next
+    assume ?b
+    then have \<open>length xs = length p\<close>
+      by (auto simp: heap_list_add_same_length mod_star_conv)
+    then show ?a
+      using \<open>?b\<close>
+        by (auto simp: heap_list_all_heap_list_all_nth)
+    qed
+  then show ?thesis
+    unfolding arrayO_except_def arrayO_def by (auto simp: ex_assn_def)
+qed
+
+lemma arrayO_except_array0_index: \<open>i < length xs \<Longrightarrow> arrayO_except R [i] xs asx (\<lambda>p. R (xs ! i) (p ! i)) = arrayO R xs asx\<close>
+  unfolding arrayO_except_array0[symmetric] arrayO_except_def
+  using heap_list_all_nth_remove1[of i \<open>[0..<length xs]\<close> R xs] by (auto simp: star_aci(2,3))
+
+lemma arrayO_nth_rule:
+  assumes i: \<open>i < length a\<close>
+  shows \<open> <arrayO (arl_assn R) a ai> Array.nth ai i <\<lambda>r. arrayO_except (arl_assn R) [i] a ai
+   (\<lambda>r'. arl_assn R (a ! i) r * \<up>(r = r' ! i))>\<close>
+proof -
+  have i_le: \<open>i < Array.length h ai\<close> if \<open>(h, as) \<Turnstile> arrayO (arl_assn R) a ai\<close> for h as
+    using  that i unfolding arrayO_def array_assn_def is_array_def
+    by (auto simp: run.simps tap_def arrayO_def
+        mod_star_conv array_assn_def is_array_def
+        Abs_assn_inverse heap_list_add_same_length length_def snga_assn_def)
+  have A: \<open>Array.get h ai ! i = p ! i\<close> if \<open>(h, as) \<Turnstile>
+       array_assn id_assn p ai *
+       heap_list_all_nth (arl_assn R) (remove1 i [0..<length p]) a p *
+       arl_assn R (a ! i) (p ! i)\<close>
+    for as p h
+    using that
+    by (auto simp: mod_star_conv array_assn_def is_array_def Array.get_def snga_assn_def
+        Abs_assn_inverse)
+  show ?thesis
+    unfolding hoare_triple_def Let_def
+    apply (clarify, intro allI impI conjI)
+    using assms A
+       apply (auto simp: hoare_triple_def Let_def i_le execute_simps relH_def in_range.simps
+        arrayO_except_array0_index[of i, symmetric]
+        elim!: run_elims
+        intro!: norm_pre_ex_rule)
+    apply (auto simp: arrayO_except_def)
+    done
+qed
 
 definition nth_aa where
   \<open>nth_aa xs i j = do {
@@ -63,87 +183,17 @@ lemma nth_aa_hnr[sepref_fr_rules]:
 proof -
   obtain R' where R: \<open>the_pure R = R'\<close> and R': \<open>R = pure R'\<close>
     using p by fastforce
-  have [simp]: \<open>(\<exists>\<^sub>Ax. arrayO (arl_assn R) a ai * R x r * true * \<up> (x = a ! ba ! b)) =
-     (arrayO (arl_assn R) a ai * R (a ! ba ! b) r * true)\<close> for a ai ba b r
-    by (auto simp: ex_assn_def)
+  have H: \<open>list_all2 (\<lambda>x x'. (x, x') \<in> the_pure (\<lambda>a c. \<up> ((c, a) \<in> R'))) bc (a ! ba) \<Longrightarrow> b < length (a ! ba) \<Longrightarrow>
+       (bc ! b, a ! ba ! b) \<in> R'\<close> for bc a ba b
+    by (auto simp add: ent_refl_true list_all2_conv_all_nth is_pure_alt_def pure_app_eq[symmetric])
   show ?thesis
-  proof (sepref_to_hoare, clarsimp simp only: hoare_triple_def Let_def, intro allI impI conjI)
-    fix a :: \<open>'a list list\<close> and ai :: \<open>('b array_list) array\<close> and
-      h :: Heap.heap and as:: \<open>nat set\<close> and \<sigma> :: \<open>Heap.heap option\<close> and r :: 'b and
-      i i' j j' :: nat
-    assume
-      i: \<open>i < length a\<close> and
-      j: \<open>j < length (a ! i)\<close> and
-      h: \<open> (h, as) \<Turnstile>
-       \<up> ((j', j) \<in> nat_rel) * \<up> ((i', i) \<in> nat_rel) *
-       arrayO (arl_assn R) a ai\<close> and
-      run: \<open>run (nth_aa ai i' j') (Some h) \<sigma> r\<close>
-
-    have i_le: \<open>i < Array.length h ai\<close>
-      using h i unfolding arrayO_def array_assn_def is_array_def
-      by (auto simp: run.simps tap_def arrayO_def
-          mod_star_conv array_assn_def is_array_def
-          Abs_assn_inverse heap_list_add_same_length length_def snga_assn_def)
-    have xs_i: \<open>\<exists>as'. (h, as') \<Turnstile> (arl_assn R) (a ! i) (Array.get h ai ! i)\<close>
-      using h i unfolding arrayO_def array_assn_def is_array_def
-      using models_heap_list_all_models_nth[of _ _ _ _ _ i]
-      by (auto simp: run.simps tap_def arrayO_def
-          mod_star_conv array_assn_def is_array_def
-          Abs_assn_inverse heap_list_add_same_length length_def snga_assn_def)
-    then have j_le_get: \<open>j < Array.length h (fst (Array.get h ai ! i))\<close>
-      using j unfolding arrayO_def arl_assn_def is_array_list_def
-      by (cases \<open>Array.get h ai ! i\<close>) (auto simp: run.simps tap_def arrayO_def hr_comp_def
-          mod_star_conv array_assn_def is_array_def
-          Abs_assn_inverse heap_list_add_same_length length_def snga_assn_def
-          dest: list_rel_pres_length)
-    have j_le_get_snd: \<open>j < snd (Array.get h ai ! i)\<close>
-      using j xs_i unfolding arrayO_def arl_assn_def is_array_list_def
-      by (cases \<open>Array.get h ai ! i\<close>) (auto simp: run.simps tap_def arrayO_def hr_comp_def
-          mod_star_conv array_assn_def is_array_def
-          Abs_assn_inverse heap_list_add_same_length length_def snga_assn_def
-          dest: list_rel_pres_length)
-    have ex_arl: \<open>execute (arl_get (Array.get h ai ! i) j) h =
-        Some (Array.get h (fst (Array.get h ai ! i)) ! j, h)\<close>
-      using run h assms i_le i j j_le_get
-      by (auto simp: run.simps tap_def arrayO_def execute_simps
-          mod_star_conv array_assn_def is_array_def nth_aa_def Array.nth_def
-          Abs_assn_inverse heap_list_add_same_length snga_assn_def
-           arl_get_def split_beta
-          split: option.splits)
-    have ex: \<open>execute (nth_aa ai i j) h = Some (Array.get h (fst (Array.get h ai ! i)) ! j, h)\<close>
-      using run h assms i_le
-      by (auto simp: run.simps tap_def arrayO_def execute_simps ex_arl
-          mod_star_conv array_assn_def is_array_def nth_aa_def Array.nth_def
-          Abs_assn_inverse heap_list_add_same_length length_def snga_assn_def
-          execute_bind_case split: option.splits)
-    show \<open>\<not> is_exn \<sigma>\<close>
-      using run h assms
-      by (auto simp: run.simps tap_def arrayO_def execute_simps ex
-          mod_star_conv array_assn_def is_array_def Array.nth_def
-          Abs_assn_inverse heap_list_add_same_length length_def snga_assn_def)
-    show \<open>(the_state \<sigma>, new_addrs h as (the_state \<sigma>)) \<Turnstile>
-       \<up> ((j', j) \<in> nat_rel) * \<up> ((i', i) \<in> nat_rel) * arrayO (arl_assn R) a ai *
-            (\<exists>\<^sub>Ax. R x r * \<up> (RETURN x \<le> RETURN (nth_ll a i j))) * true\<close>
-      using run h assms xs_i j_le_get i_le j_le_get_snd
-      apply (cases \<open>Array.get h ai ! i\<close>)
-      apply (auto simp: run.simps tap_def arrayO_def R R' nth_ll_def
-          mod_star_conv arl_assn_def is_array_list_def hr_comp_def ex list_rel_def
-          Abs_assn_inverse heap_list_add_same_length length_def snga_assn_def
-          dest!: list_all2_nthD[of _ _ _ j])
-        by blast
-    show \<open>relH {a. a < lim h \<and> a \<notin> as} h (the_state \<sigma>)\<close>
-      using run h assms xs_i
-      by (auto simp: run.simps tap_def arrayO_def
-          mod_star_conv arl_assn_def is_array_list_def hr_comp_def ex list_rel_def
-          Abs_assn_inverse heap_list_add_same_length length_def snga_assn_def relH_def
-          in_range.simps)
-    show \<open>lim h \<le> lim (the_state \<sigma>)\<close>
-      using run h assms xs_i
-      by (auto simp: run.simps tap_def arrayO_def
-          mod_star_conv arl_assn_def is_array_list_def hr_comp_def ex list_rel_def
-          Abs_assn_inverse heap_list_add_same_length length_def snga_assn_def relH_def
-          in_range.simps)
-  qed
+  apply sepref_to_hoare
+  apply (subst (2) arrayO_except_array0_index[symmetric])
+    apply (solves \<open>auto\<close>)[]
+  apply (sep_auto simp: nth_aa_def nth_ll_def intro!: arrayO_nth_rule)
+  apply (sep_auto simp: arrayO_except_def arrayO_def arl_assn_def hr_comp_def list_rel_def list_all2_lengthD
+      star_aci(3) R R' pure_def H)
+    done
 qed
 
 definition update_aa where
@@ -171,7 +221,8 @@ lemma
    apply (auto simp: execute_simps execute_bind_case Array.nth_def
       Array.upd_def
       split: option.splits)
-    oops
+  oops
+declare arrayO_nth_rule[sep_heap_rules]
 lemma nth_aa_hnr[sepref_fr_rules]:
   fixes R ::  \<open>'a \<Rightarrow> 'b :: {heap, default}\<Rightarrow> assn\<close>
   assumes p: \<open>is_pure R\<close>
@@ -186,7 +237,15 @@ proof -
     by (auto simp: ex_assn_def)
   have ?thesis
     apply sepref_to_hoare
-    apply (auto simp: append_el_aa_def (* arrayO_def *) array_assn_def is_array_def)
+    apply (sep_auto simp: append_el_aa_def)
+     apply (sep_auto simp:  arrayO_except_def arl_append_def arl_assn_def (* is_array_list_def *)
+        (* arrayO_def *) (* arl_assn_def *) (* is_array_def *)
+        hr_comp_def eq_commute[of \<open>(_, _)\<close>])
+      
+     apply (sep_auto simp: arrayO_except_def arrayO_def arl_assn_def (* is_array_def *)
+        hr_comp_def eq_commute[of \<open>(_, _)\<close>])
+      thm upd_rule
+      thm arl_append_rule
     apply (rule bind_rule)
       -- \<open>some work on ArrayO missing\<close>
       sorry
